Use a keyed hash functionality and a few neat tricks to make this interface nice to use

experiments/Veritas.HashSet.fst
@@ -20,25 +20,37 @@ let flush_interleaving = ()
 open LowStar.BufferOps
 
 // Relying on a somewhat recent kremlin optimization that removes pointers to unit
-let state_s =
-  Hacl.Hash.Definitions.hash_t Spec.Hash.Definitions.SHA2_256 & B.pointer (G.erased (list hashable_bytes))
+noeq
+type state_s = {
+  acc: acc:B.buffer u8 { B.length acc == 64 };
+  seen: B.pointer (G.erased (list hashable_bytes));
+  key: key:B.buffer u8 { B.length key == 64 };
+  g_key: G.erased t_key;
+}
 
 let seen h s =
-  let _, p = B.deref h s in
-  G.reveal (B.deref h p)
+  let s = B.deref h s in
+  G.reveal (B.deref h s.seen)
 
 let v h s =
-  let b, _ = B.deref h s in
-  B.as_seq h b
+  let s = B.deref h s in
+  B.as_seq h s.acc
 
-let footprint_s (b, p) =
-  B.(loc_addr_of_buffer b `loc_union` loc_addr_of_buffer p)
+let key s =
+  G.reveal s.g_key
 
-let invariant_s h (b, p) =
-  B.live h b /\ B.freeable b /\
-  B.live h p /\ B.freeable p /\
-  B.as_seq h b == gfold_right fold_and_hash (G.reveal (B.deref h p)) zero /\
-  B.disjoint b p
+let footprint_s s =
+  B.(loc_addr_of_buffer s.acc `loc_union` loc_addr_of_buffer s.seen `loc_union` loc_addr_of_buffer s.key)
+
+let invariant_s h s =
+  B.live h s.acc /\ B.freeable s.acc /\
+  B.live h s.seen /\ B.freeable s.seen /\
+  B.live h s.key /\ B.freeable s.key /\
+  B.disjoint s.acc s.seen /\
+  B.disjoint s.acc s.key /\
+  B.disjoint s.seen s.key /\
+  B.as_seq h s.acc == gfold_right (fold_and_hash s.g_key) (G.reveal (B.deref h s.seen)) zero /\
+  G.reveal s.g_key == B.as_seq h s.key
 
 let invariant_loc_in_footprint _ _ =
   allow_inversion state_s
@@ -50,10 +62,17 @@ let frame _ _ _ _ =
   allow_inversion state_s
 
 #push-options "--ifuel 1 --fuel 1 --z3rlimit 50"
-let create_in r =
-  let b = B.malloc r (Lib.IntTypes.u8 0) 32ul in
-  let p = B.malloc r (G.hide []) 1ul in
-  B.malloc r (b, p) 1ul
+let create_in r k' =
+  let h0 = ST.get () in
+  let b = B.malloc r (Lib.IntTypes.u8 0) 64ul in
+  let p = B.malloc r (G.hide ([] #hashable_bytes)) 1ul in
+  let k = B.malloc r (Lib.IntTypes.u8 0) 64ul in
+  B.blit k' 0ul k 0ul 64ul;
+  let h1 = ST.get () in
+  B.modifies_only_not_unused_in B.loc_none h0 h1;
+  [@inline_let]
+  let s: state_s = { acc = b; seen = p; key = k; g_key = B.as_seq h0 k' } in
+  B.malloc r s 1ul
 #pop-options
 
 assume val xor_inplace (b1: B.buffer u8) (b2: B.buffer u8): Stack unit
@@ -64,24 +83,48 @@ assume val xor_inplace (b1: B.buffer u8) (b2: B.buffer u8): Stack unit
     B.(modifies (loc_buffer b1) h0 h1) /\
     B.as_seq h1 b1 == xor_bytes (B.as_seq h0 b1) (B.as_seq h0 b2)))
 
-#push-options "--fuel 1 --z3rlimit 100"
+inline_for_extraction noextract
+let why (x: B.buffer u8) (l: UInt32.t { B.len x == l }): y:Lib.Buffer.lbuffer u8 l = x
+
+#push-options "--fuel 1 --z3rlimit 200"
 let add s b l =
   let _ = allow_inversion state_s in
   let h0 = ST.get () in
   assert (invariant h0 s);
   push_frame ();
-  let acc, p = !* s in
+  let { acc; seen; key } = !* s in
   let h1 = ST.get () in
   assert (invariant h1 s);
-  let tmp = B.alloca (Lib.IntTypes.u8 0) 32ul in
-  Hacl.Hash.SHA2.hash_256 b l tmp;
+  let tmp = B.alloca (Lib.IntTypes.u8 0) 64ul in
+  assert_norm (64 + Spec.Blake2.(size_block Blake2B) < pow2 32);
+  assert_norm (64 < pow2 32);
+  assert_norm (64 <= Spec.Blake2.(max_key Blake2B));
+  assert (B.length tmp == 64);
+  [@inline_let]
+  let tmp = why tmp 64ul in
+  [@inline_let]
+  let key = why key 64ul in
+  Hacl.Blake2b_32.blake2b 64ul tmp l b 64ul key;
   xor_inplace acc tmp;
-  p *= G.hide (B.as_seq h1 b :: B.deref h1 p);
+  seen *= G.hide (B.as_seq h1 b :: B.deref h1 seen);
+  let h5 = ST.get () in
+  assert (
+    let h = h5 in
+    let s = B.deref h5 s in
+    B.live h s.acc /\ B.freeable s.acc /\
+    B.live h s.seen /\ B.freeable s.seen /\
+    B.live h s.key /\ B.freeable s.key /\
+    B.disjoint s.acc s.seen /\
+    B.disjoint s.acc s.key /\
+    B.disjoint s.seen s.key /\
+    B.as_seq h s.acc == gfold_right (fold_and_hash s.g_key) (G.reveal (B.deref h s.seen)) zero /\
+    G.reveal s.g_key == B.as_seq h s.key);
   pop_frame ()
 #pop-options
 
 let free s =
-  let acc, p = !* s in
+  let { seen; acc; key } = !* s in
   B.free s;
+  B.free seen;
   B.free acc;
-  B.free p
+  B.free key
